Changes in specification for uint63 to unsigned; add spec/proof for uint63_add

examples/uint63nat/specs.v
@@ -108,10 +108,9 @@ Definition args_make_Coq_Init_Datatypes_nat_S_spec : ident * funspec :=
 DECLARE _get_args
         (args_spec_S').
 
-(* Same as in UVRooster - TODO: encode_Z as relation to fit our general scheme *)
+(* Same as in UVRooster 
+- TODO: encode_Z as relation to fit our general scheme *)
 Definition encode_Z (x: Z): Z := x * 2 + 1.
-Definition min_signed: Z := - 2^62.
-Definition max_signed: Z := 2^62 - 1.
 
 #[export] Instance CompSpecs : compspecs. make_compspecs prog. Defined.
 
@@ -128,18 +127,18 @@ Definition uint63_to_nat_spec :  ident *  funspec :=
         ti : val, outlier : outlier_t, t_info : GCGraph.thread_info
    PRE  [ tptr (Tstruct _thread_info noattr ),  (talignas 3%N (tptr tvoid)) ]
       PROP (  writable_share sh; 
-            min_signed <= encode_Z (Z.of_nat n) <= max_signed
+            encode_Z (Z.of_nat n) <= Int64.max_unsigned
             )
       PARAMS (ti; Vlong (Int64.repr (encode_Z (Z.of_nat n))))
       GLOBALS (gv)
-      SEP (full_gc g t_info roots outlier ti sh gv; library.mem_mgr gv)
+      SEP (full_gc g t_info roots outlier ti sh gv; VST.floyd.library.mem_mgr gv)
    POST [ (talignas 3%N (tptr tvoid)) ]
      EX (p' : rep_type) (g' : graph) (t_info' : GCGraph.thread_info) (roots': roots_t),
        PROP (@is_in_graph nat (@in_graph nat _) g' outlier n p' ;
              gc_graph_iso g roots g' roots';
              frame_shells_eq (ti_frames t_info) (ti_frames t_info'))
        RETURN  (rep_type_val g' p')
-       SEP (full_gc g' t_info' roots' outlier ti sh gv; library.mem_mgr gv). 
+       SEP (full_gc g' t_info' roots' outlier ti sh gv; VST.floyd.library.mem_mgr gv). 
 
 Definition uint63_to_nat_no_gc_spec :  ident *  funspec := 
 DECLARE _uint63_to_nat_no_gc
@@ -148,7 +147,7 @@ WITH gv : globals, g : graph, roots : roots_t, sh : share, n: nat,
 PRE  [ tptr (Tstruct _thread_info noattr ),  (talignas 3%N (tptr tvoid)) ]
     PROP ( 2 * (Z.of_nat n) < headroom t_info ; 
           writable_share sh; 
-          min_signed <= encode_Z (Z.of_nat n) <= max_signed
+          encode_Z (Z.of_nat n) <= Int64.max_unsigned
           )
     PARAMS (ti; Vlong (Int64.repr (encode_Z (Z.of_nat n))))
     GLOBALS (gv)
@@ -165,7 +164,7 @@ DECLARE _uint63_from_nat
 WITH gv : globals, g : graph, roots : roots_t, sh : share, n: nat, p : rep_type,
         ti : val, outlier : outlier_t, t_info : GCGraph.thread_info
 PRE  [ int_or_ptr_type ]
-    PROP ( encode_Z (Z.of_nat n) <= max_signed; 
+    PROP ( encode_Z (Z.of_nat n) <= Int64.max_signed; 
             @is_in_graph nat (@in_graph nat _) g outlier n p ;
             writable_share sh)
     PARAMS (rep_type_val g p)
@@ -176,6 +175,23 @@ POST [ int_or_ptr_type ]
     RETURN  (Vlong (Int64.repr (encode_Z (Z.of_nat n))))
     SEP (full_gc g t_info roots outlier ti sh gv). 
     (* KS: Existential *)
+
+Definition uint63_add_spec : ident * funspec := 
+  DECLARE _uint63_add 
+  WITH m : nat, n : nat 
+PRE [ int_or_ptr_type, int_or_ptr_type ]
+  PROP (encode_Z (Z.of_nat m) <= Int64.max_unsigned;
+        encode_Z (Z.of_nat n) <= Int64.max_unsigned; 
+        encode_Z (Z.of_nat (m + n)) <= Int64.max_unsigned
+        ) 
+  PARAMS (Vlong (Int64.repr (encode_Z (Z.of_nat m)));
+           Vlong (Int64.repr (encode_Z (Z.of_nat n)))) 
+  GLOBALS () 
+  SEP () 
+POST [ int_or_ptr_type ]
+  PROP ()
+  RETURN (Vlong (Int64.repr (encode_Z (Z.of_nat (m + n)))))
+  SEP ().
 
 (* Function Spec
 
@@ -265,10 +281,12 @@ POST [ int_or_ptr_type ]
 	SEP (full_gc g' t_info' roots outlier ti sh gv).
 
 
+
 Definition Vprog : varspecs. mk_varspecs prog. Defined.
 Definition Gprog := [ tag_spec_S; alloc_make_Coq_Init_Datatypes_nat_O_spec; alloc_make_Coq_Init_Datatypes_nat_S_spec
                       ; args_make_Coq_Init_Datatypes_nat_S_spec ;  uint63_to_nat_spec ; uint63_from_nat_spec; 
                       uint63_to_nat_no_gc_spec;
-                      gc_spec.garbage_collect_spec
+                      gc_spec.garbage_collect_spec;
+                      uint63_add_spec
                       (* _call, call_spec *)
                       ] .
